@base  <http://www.idpf.org/epub/vocab/structure/> .
@prefix rdf:  <http://www.w3.org/1999/02/22-rdf-syntax-ns#> .
@prefix rdfs: <http://www.w3.org/2000/01/rdf-schema#> .
@prefix owl:  <http://www.w3.org/2002/07/owl#> .
@prefix zt:  <http://www.daisy.org/ns/rdf/property#> .
@prefix htu: <http://www.daisy.org/ns/rdf/usage/html/#> .
@prefix mou: <http://www.daisy.org/ns/rdf/usage/media-overlays/#> .
@prefix dcterms:  <http://purl.org/dc/terms/> .
@prefix jena: <http://www.daisy.org/ns/rdf/jena#> .
@prefix foaf: <http://xmlns.com/foaf/spec/#term_> .
@prefix aria: <http://www.w3.org/WAI/ARIA/schemata/aria-1.rdf#> .
@prefix xhv: <http://www.w3.org/1999/xhtml/vocab/#> .
@prefix role: <http://www.w3.org/1999/xhtml/vocab#> .
@prefix epub: <http://www.idpf.org/epub/vocab#> .
@prefix : <#> .

<>
  dcterms:title "EPUB 3 Structural Semantics Vocabulary" ;
  dcterms:description "This vocabulary, a part of EPUB® 3, defines a set of properties relating to the description of structural semantics of written works. While the vocabulary is generally host language agnostic, it has been constructed primarily to enable semantic inflection of elements in the HTML vocabulary." ;
  dcterms:publisher "International Digital Publishing Forum (IDPF)" ;
  dcterms:issued "2014-06-28" ; 
  dcterms:creator "mgylling" ; 
  dcterms:creator "mgarrish" .
  

########## partitions #########

:partitions                                a rdf:Bag ;
					                       jena:bag-sort "10" ;
					                       dcterms:title "Document partitions" .
					
:cover                                     a rdf:Property ;
					                       rdfs:label "cover";
					                       rdf:member :partitions ;
					                       htu:usage "[[http://www.w3.org/TR/html5/sections.html#the-section-element section]], [[http://www.w3.org/TR/html5/sections.html#the-body-element-0 body]]" ;
					                       jena:prop-sort "10" ;
					                       rdfs:comment "A section that introduces the work, often consisting of a marketing image, the title, author and publisher, and select quotes and reviews." .							

:frontmatter                               a rdf:Property ;
					                       rdfs:label "frontmatter";
					                       rdf:member :partitions ;
					                       htu:usage "[[http://www.w3.org/TR/html5/sections.html#the-section-element section]], [[http://www.w3.org/TR/html5/sections.html#the-body-element-0 body]]" ;
					                       jena:prop-sort "20" ;
					                       rdfs:comment "Preliminary material to the main content of a publication, such as tables of contents, dedications, etc." .

:bodymatter                                a rdf:Property ;
					                       rdfs:label "bodymatter";
					                       rdf:member :partitions ;
					                       htu:usage "[[http://www.w3.org/TR/html5/sections.html#the-section-element section]], [[http://www.w3.org/TR/html5/sections.html#the-body-element-0 body]]" ;
					                       jena:prop-sort "30" ;
					                       rdfs:comment "The main content of a publication." .

:backmatter                                a rdf:Property ;
					                       rdfs:label "backmatter";
					                       rdf:member :partitions ;
					                       htu:usage "[[http://www.w3.org/TR/html5/sections.html#the-section-element section]], [[http://www.w3.org/TR/html5/sections.html#the-body-element-0 body]]" ;
					                       jena:prop-sort "40" ;
					                       rdfs:comment "Ancillary material occurring after the main content of a publication, such as indices, appendices, etc." .



########## divisions #########

:divisions                                  a rdf:Bag ;
                                            jena:bag-sort "20" ;
                                            dcterms:title "Document divisions" .

:volume                                     a rdf:Property ;
                                            rdfs:label "volume";
                                            rdf:member :divisions ;
                                            htu:usage "[[http://www.w3.org/TR/html5/sections.html#the-section-element section]], [[http://www.w3.org/TR/html5/sections.html#the-body-element-0 body]]" ;
                                            jena:prop-sort "10" ;
                                            rdfs:comment "A component of a collection." .

:part                                       a rdf:Property;
                                            rdfs:label "part";
                                            rdf:member :divisions ;
                                            htu:usage "[[http://www.w3.org/TR/html5/sections.html#the-section-element section]], [[http://www.w3.org/TR/html5/sections.html#the-body-element-0 body]]" ;
                                            jena:prop-sort "20" ;
                                            rdfs:comment "A major structural division in a work that contains a set of related sections dealing with a particular subject, narrative arc or similar encapsulated theme." .

:chapter                                    a rdf:Property ;
					                        rdfs:label "chapter";
                                            rdf:member :divisions ;
                                            htu:usage "[[http://www.w3.org/TR/html5/sections.html#the-section-element section]], [[http://www.w3.org/TR/html5/sections.html#the-body-element-0 body]]" ;
                                            jena:prop-sort "30" ;
                                            rdfs:comment "A major thematic section of content in a work." .

:subchapter                                 a rdf:Property ;
                                            rdfs:label "subchapter";
                                            rdf:member :divisions ;
                                            htu:usage "[[http://www.w3.org/TR/html5/sections.html#the-section-element section]], [[http://www.w3.org/TR/html5/sections.html#the-body-element-0 body]]" ;
                                            jena:prop-sort "40" ;
                                            rdfs:comment "A major sub-division of a chapter." .

:division                                   a rdf:Property ;
                                            rdfs:label "division";
                                            rdf:member :divisions ;
                                            htu:usage "[[http://www.w3.org/TR/html5/sections.html#the-section-element section]], [[http://www.w3.org/TR/html5/sections.html#the-body-element-0 body]]" ;
                                            jena:prop-sort "50" ;
                                            rdfs:comment "A major structural division that may also appear as a substructure of a part (esp. in legislation)." .

#:section                                   a rdf:Property ;
#                                           rdfs:label "section";
#                                           rdf:member :divisions ;
#                                           rdfs:comment "A structural division typically subordinate in importance to a part or division (esp. in textbooks and legislation)." .
#
#:subsection                                a rdf:Property ;
#                                           rdfs:label "subsection";
#                                           rdf:member :divisions ;
#                                           rdfs:comment "A major sub-division of a section." .


########## sections #########

:sections                                   a rdf:Bag ;
					                        jena:bag-sort "30" ;
					                        dcterms:title "Document sections and components" ;
					                        dcterms:description "Sections and components that typically occur in the publication bodymatter." .

:abstract                                   a rdf:Property ;
                                            rdfs:label "abstract";
                                            rdf:member :sections ;
                                            htu:usage "[[http://www.w3.org/TR/html5/sections.html#the-section-element section]], [[http://www.w3.org/TR/html5/grouping-content.html#grouping-content grouping content]]" ;
                                            jena:prop-sort "5" ;
                                            rdfs:comment "A short summary of the principle ideas, concepts and conclusions of the work, or of a section or excerpt within it." ;
                                            epub:status "draft" .

:foreword                                   a rdf:Property ;
                                            rdfs:label "foreword";
                                            rdf:member :sections ;
                                            htu:usage "[[http://www.w3.org/TR/html5/sections.html#the-section-element section]], [[http://www.w3.org/TR/html5/grouping-content.html#grouping-content grouping content]]" ;
                                            jena:prop-sort "10" ;
                                            rdfs:comment "An introductory section that precedes the work, typically not written by the author of the work." .

:preface                                    a rdf:Property ;
                                            rdfs:label "preface";
                                            rdf:member :sections ;
                                            htu:usage "[[http://www.w3.org/TR/html5/sections.html#the-section-element section]], [[http://www.w3.org/TR/html5/grouping-content.html#grouping-content grouping content]]" ;
                                            jena:prop-sort "20" ;
                                            rdfs:comment "An introductory section that precedes the work, typically written by the author of the work." .

:prologue                                   a rdf:Property ;
                                            rdfs:label "prologue" ;
                                            rdf:member :sections ;
                                            htu:usage "[[http://www.w3.org/TR/html5/sections.html#the-section-element section]], [[http://www.w3.org/TR/html5/grouping-content.html#grouping-content grouping content]]" ;
                                            jena:prop-sort "30" ;
                                            rdfs:comment "An introductory section that sets the background to a work, typically part of the narrative." .

:introduction                               a rdf:Property ;
                                            rdfs:label "introduction";
                                            rdf:member :sections ;
                                            htu:usage "[[http://www.w3.org/TR/html5/sections.html#the-section-element section]], [[http://www.w3.org/TR/html5/grouping-content.html#grouping-content grouping content]]" ;
                                            jena:prop-sort "40" ;
                                            rdfs:comment "A preliminary section that typically introduces the scope or nature of the work.".

:preamble                                   a rdf:Property ;
                                            rdfs:label "preamble" ;
                                            rdf:member :sections ;
                                            htu:usage "[[http://www.w3.org/TR/html5/sections.html#the-section-element section]], [[http://www.w3.org/TR/html5/grouping-content.html#grouping-content grouping content]]" ;
                                            jena:prop-sort "50" ;
                                            rdfs:comment "A section in the beginning of the work, typically containing introductory and/or explanatory prose regarding the scope or nature of the work's content".

:qna                                        a rdf:Property ;
                                            rdfs:label "qna" ;
                                            rdf:member :testing ;
                                            htu:usage "lists or [[http://www.w3.org/TR/html5/dom.html#sectioning-content-0 sectioning content]]" ;
                                            jena:prop-sort "70" ;
                                            rdfs:comment "A section of content structured as a series of questions and answers, such as an interview or list of frequently asked questions." .

:conclusion                                 a rdf:Property ;
                                            rdfs:label "conclusion" ;
                                            rdf:member :sections ;
                                            htu:usage "[[http://www.w3.org/TR/html5/sections.html#the-section-element section]], [[http://www.w3.org/TR/html5/grouping-content.html#grouping-content grouping content]]" ;
                                            jena:prop-sort "60" ;
                                            rdfs:comment "A concluding section or statement that summarizes the work or wraps up the narrative." .

:epilogue                                   a rdf:Property ;
                                            rdfs:label "epilogue" ;
                                            rdf:member :sections ;
                                            htu:usage "[[http://www.w3.org/TR/html5/sections.html#the-section-element section]], [[http://www.w3.org/TR/html5/grouping-content.html#grouping-content grouping content]]" ;
                                            jena:prop-sort "70" ;
                                            rdfs:comment "A concluding section of narrative that wraps up or comments on the actions and events of the work, typically from a future perspective." .

:afterword		                            a rdf:Property ;
                                            rdfs:label "afterword" ;
                                            rdf:member :sections ;
                                            htu:usage "[[http://www.w3.org/TR/html5/sections.html#the-section-element section]], [[http://www.w3.org/TR/html5/grouping-content.html#grouping-content grouping content]]" ;
                                            jena:prop-sort "80" ;
                                            rdfs:comment "A closing statement from the author or a person of importance, typically providing insight into how the content came to be written, its significance, or related events that have transpired since its timeline." .

:epigraph                                   a rdf:Property ;
                                            rdfs:label "epigraph" ;
                                            rdf:member :sections ;
                                            htu:usage "[[http://www.w3.org/TR/html5/sections.html#the-section-element section]], [[http://www.w3.org/TR/html5/grouping-content.html#grouping-content grouping content]]" ;
                                            jena:prop-sort "90" ;
                                            rdfs:comment "A quotation set at the start of the work or a section that establishes the theme or sets the mood." .



########### navigation ###########

:navigation                                 a rdf:Bag ;
                                            jena:bag-sort "35" ;
                                            dcterms:title "Document navigation" .


:toc                                        a rdf:Property ;
                                            rdfs:label "toc" ;
                                            rdf:member :navigation ;
                                            htu:usage "[[http://www.w3.org/TR/html5/dom.html#sectioning-content-0 sectioning content]]" ;
                                            jena:prop-sort "10" ;
                                            rdfs:comment "A navigational aid that provides an ordered list of links to the major sectional headings in the content. A table of contents may cover an entire work, or only a smaller section of it." .

:toc-brief                                  a rdf:Property ;
                                            rdfs:label "toc-brief" ;
                                            rdf:member :navigation ;
                                            htu:usage "[[http://www.w3.org/TR/html5/dom.html#sectioning-content-0 sectioning content]]" ;
                                            jena:prop-sort "20" ;
                                            rdfs:comment "An abridged version of the table of contents." ;
                                            epub:status "draft" .

:landmarks                                  a rdf:Property ;
                                            rdfs:label "landmarks" ;
                                            rdf:member :navigation ;
                                            htu:usage "[[http://www.w3.org/TR/html5/dom.html#sectioning-content-0 sectioning content]]" ;
                                            jena:prop-sort "25" ;
                                            rdfs:comment "A collection of references to well-known/recurring components within the publication" .

:loa                                        a rdf:Property ;
                                            rdfs:label "loa" ;
                                            rdf:member :navigation ;
                                            htu:usage "[[http://www.w3.org/TR/html5/dom.html#sectioning-content-0 sectioning content]]" ;
                                            jena:prop-sort "30" ;
                                            rdfs:comment "A listing of audio clips included in the work." .

:loi                                        a rdf:Property ;
                                            rdfs:label "loi" ;
                                            rdf:member :navigation ;
                                            htu:usage "[[http://www.w3.org/TR/html5/dom.html#sectioning-content-0 sectioning content]]" ;
                                            jena:prop-sort "40" ;
                                            rdfs:comment "A listing of illustrations included in the work." .

:lot                                        a rdf:Property ;
                                            rdfs:label "lot" ;
                                            rdf:member :navigation ;
                                            htu:usage "[[http://www.w3.org/TR/html5/dom.html#sectioning-content-0 sectioning content]]" ;
                                            jena:prop-sort "50" ;
                                            rdfs:comment "A listing of tables included in the work." .

:lov                                        a rdf:Property ;
                                            rdfs:label "lov" ;
                                            rdf:member :navigation ;
                                            htu:usage "[[http://www.w3.org/TR/html5/dom.html#sectioning-content-0 sectioning content]]" ;
                                            jena:prop-sort "60" ;
                                            rdfs:comment "A listing of video clips included in the work." .



########## reference sections #########


:references                                 a rdf:Bag ;
                                            jena:bag-sort "40" ;
                                            dcterms:title "Document reference sections" .

:appendix                                   a rdf:Property ;
                                            rdfs:label "appendix" ;
                                            rdf:member :references ;
                                            htu:usage "[[http://www.w3.org/TR/html5/dom.html#sectioning-content-0 sectioning content]]" ;
                                            jena:prop-sort "10" ;
                                            rdfs:comment "A section of supplemental information located after the primary content that informs the content but is not central to it." .

:colophon                                   a rdf:Property ;
                                            rdfs:label "colophon" ;
                                            rdf:member :references ;
                                            htu:usage "[[http://www.w3.org/TR/html5/dom.html#sectioning-content-0 sectioning content]], [[http://www.w3.org/TR/html5/grouping-content.html#grouping-content grouping content]]" ;
                                            jena:prop-sort "20" ;
                                            rdfs:comment "A short section of production notes particular to the edition (e.g., describing the typeface used), often located at the end of a work." .

:credits                                    a rdf:Property ;
                                            rdfs:label "credits" ;
                                            htu:usage "[[http://www.w3.org/TR/html5/dom.html#sectioning-content-0 sectioning content]], [[http://www.w3.org/TR/html5/grouping-content.html#grouping-content grouping content]]" ;
                                            rdf:member :references ;
                                            jena:prop-sort "30" ;
                                            rdfs:comment "A collection of [[#credit credits]]." ;
                                            epub:status "draft" .

:keywords                                   a rdf:Property ;
                                            rdfs:label "keywords" ;
                                            htu:usage "[[http://www.w3.org/TR/html5/dom.html#sectioning-content-0 sectioning content]], [[http://www.w3.org/TR/html5/grouping-content.html#grouping-content grouping content]]" ;
                                            rdf:member :references ;
                                            jena:prop-sort "40" ;
                                            rdfs:comment "A collection of [[#keyword keywords]]."  ;
                                            epub:status "draft" .


########### indexes ###########

:indexes                                    a rdf:Bag ;
                                            jena:bag-sort "41" ;
                                            rdf:member :references ;
                                            dcterms:title "Indexes" .


:index                                      a rdf:Property ;
                                            jena:prop-sort "10" ;
                                            rdfs:label "index" ;
                                            rdf:member :indexes ;
                                            htu:usage "[[http://www.w3.org/TR/html5/dom.html#sectioning-content-0 sectioning content]], [[http://www.w3.org/TR/html5/sections.html#the-body-element-0 body]]" ;
                                            epub:usage "[[http://www.idpf.org/epub/idx/epub-indexes.html#bb-index EPUB Indexes – index property]]" ;
                                            rdfs:comment "A navigational aid that provides a detailed list of links to key subjects, names and other important topics covered in the work." .

:index-headnotes                            a rdf:Property ;
                                            jena:prop-sort "20" ;
                                            rdfs:label "index-headnotes" ;
                                            rdf:member :indexes ;
                                            role:scope :index ;
                                            htu:usage "[[http://www.w3.org/TR/html5/dom.html#sectioning-content-0 sectioning content]], [[http://www.w3.org/TR/html5/sections.html#the-header-element header]]" ;
                                            epub:usage "[[http://www.idpf.org/epub/idx/epub-indexes.html#bb-headnotes EPUB Indexes – index-headnotes property]]" ;
                                            rdfs:comment "Narrative or other content to assist users in using the index." .

:index-legend                               a rdf:Property ;
                                            jena:prop-sort "30" ;
                                            rdfs:label "index-legend" ;
                                            rdf:member :indexes ;
                                            role:scope :index-headnotes ;
                                            htu:usage "[[http://www.w3.org/TR/html5/dom.html#sectioning-content-0 sectioning content]], [[http://www.w3.org/TR/html5/grouping-content.html#the-dl-element dl]]" ;
                                            epub:usage "[[http://www.idpf.org/epub/idx/epub-indexes.html#bb-legend EPUB Indexes – index-legend property]]" ;
                                            rdfs:comment "List of symbols, abbreviations or special formatting used in the index, and their meanings." .

:index-group                                a rdf:Property ;
                                            jena:prop-sort "40" ;
                                            rdfs:label "index-group" ;
                                            rdf:member :indexes ;
                                            role:scope :index ;
                                            htu:usage "[[http://www.w3.org/TR/html5/dom.html#sectioning-content-0 sectioning content]]" ;
                                            epub:usage "[[http://www.idpf.org/epub/idx/epub-indexes.html#bb-group EPUB Indexes – index-group property]]" ;
                                            rdfs:comment "Collection of consecutive main entries that share a common characteristic, for example the starting letter of the main entries." .

:index-entry-list                           a rdf:Property ;
                                            jena:prop-sort "50" ;
                                            rdfs:label "index-entry-list" ;
                                            rdf:member :indexes ;
                                            role:scope :index ;
                                            role:scope :index-group ;
                                            role:scope :index-entry ;
                                            htu:usage "[[http://www.w3.org/TR/html5/grouping-content.html#the-ul-element ul]]; this property is implied when the ul has an ancestor of index except within index-headnotes" ;
                                            epub:usage "[[http://www.idpf.org/epub/idx/epub-indexes.html#bb-entry-list EPUB Indexes – index-entry-list property]]" ;
                                            rdfs:comment "Collection of consecutive main entries or subentries." .

:index-entry                                a rdf:Property ;
                                            jena:prop-sort "60" ;
                                            rdfs:label "index-entry" ;
                                            rdf:member :indexes ;
                                            role:scope :index-entry-list ;
                                            htu:usage "[[http://www.w3.org/TR/html5/grouping-content.html#the-li-element li]]; this property is implied when parent ul is of type index-entry-list (implicit or explicit)" ;
                                            epub:usage "[[http://www.idpf.org/epub/idx/epub-indexes.html#bb-entry EPUB Indexes – index-entry property]]" ;
                                            rdfs:comment "One term with any attendant subentries, locators, cross references, and/or editorial note." .

:index-term                                 a rdf:Property ;
                                            jena:prop-sort "70" ;
                                            rdfs:label "index-term" ;
                                            rdf:member :indexes ;
                                            role:scope :index-entry ;
                                            role:scope :index-xref-preferred ;
                                            role:scope :index-xref-related ;
                                            htu:usage "[[http://www.w3.org/TR/html5/dom.html#phrasing-content phrasing content]]; typically [[http://www.w3.org/TR/html5/text-level-semantics.html#the-span-element span]]" ;
                                            epub:usage "[[http://www.idpf.org/epub/idx/epub-indexes.html#bb-term EPUB Indexes – index-term property]]" ;
                                            rdfs:comment "Word, phrase, string, glyph or image representing the indexable content." .

:index-editor-note                          a rdf:Property ;
                                            jena:prop-sort "80" ;
                                            rdfs:label "index-editor-note" ;
                                            rdf:member :indexes ;
                                            role:scope :index-entry ;
                                            htu:usage "[[http://www.w3.org/TR/html5/rendering.html#flow-content-0 flow content]]" ;
                                            epub:usage "[[http://www.idpf.org/epub/idx/epub-indexes.html#bb-editor-note EPUB Indexes – index-editor-note property]]" ;
                                            rdfs:comment "Editorial note pertaining to a single entry." .

:index-locator                              a rdf:Property ;
                                            jena:prop-sort "90" ;
                                            rdfs:label "index-locator" ;
                                            rdf:member :indexes ;
                                            role:scope :index-entry ;
                                            role:scope :index-locator-list ;
                                            role:scope :index-locator-range ;
                                            htu:usage "[[http://www.w3.org/TR/html5/text-level-semantics.html#the-a-element a]]; this property is implied when parent context is index-locator-list or index-locator-range" ;
                                            epub:usage "[[http://www.idpf.org/epub/idx/epub-indexes.html#bb-locator EPUB Indexes – index-locator property]]" ;
                                            rdfs:comment "A reference to an occurrence of the indexed content in the publication." .

:index-locator-list                         a rdf:Property ;
                                            jena:prop-sort "100" ;
                                            rdfs:label "index-locator-list" ;
                                            rdf:member :indexes ;
                                            role:scope :index-entry ;
                                            htu:usage "[[http://www.w3.org/TR/html5/grouping-content.html#the-ul-element ul]]" ;
                                            epub:usage "[[http://www.idpf.org/epub/idx/epub-indexes.html#bb-locator-list EPUB Indexes – index-locator-list property]]" ;
                                            rdfs:comment "Collection of sequential locators or locator ranges." .

:index-locator-range                        a rdf:Property ;
                                            jena:prop-sort "110" ;
                                            rdfs:label "index-locator-range" ;
                                            rdf:member :indexes ;
                                            role:scope :index-entry ;
                                            role:scope :index-locator-list ;
                                            htu:usage "[[http://www.w3.org/TR/html5/rendering.html#flow-content-0 flow content]]" ;
                                            epub:usage "[[http://www.idpf.org/epub/idx/epub-indexes.html#bb-locator-range EPUB Indexes – index-locator-range property]]" ;
                                            rdfs:comment "A pair of locators that connects a term to a range of content rather than a single point." .

:index-xref-preferred                       a rdf:Property ;
                                            jena:prop-sort "120" ;
                                            rdfs:label "index-xref-preferred" ;
                                            rdf:member :indexes ;
                                            role:scope :index-entry ;
                                            htu:usage "[[http://www.w3.org/TR/html5/rendering.html#flow-content-0 flow content]]" ;
                                            epub:usage "[[http://www.idpf.org/epub/idx/epub-indexes.html#bb-xref-preferred EPUB Indexes – index-xref-preferred property]]" ;
                                            rdfs:comment "Reference from one term to one or more preferred terms or term categories in an index (analogous to \"See xxx\")." .

:index-xref-related                         a rdf:Property ;
                                            jena:prop-sort "130" ;
                                            rdfs:label "index-xref-related" ;
                                            rdf:member :indexes ;
                                            role:scope :index-entry ;
                                            htu:usage "[[http://www.w3.org/TR/html5/rendering.html#flow-content-0 flow content]]" ;
                                            epub:usage "[[http://www.idpf.org/epub/idx/epub-indexes.html#bb-xref-related EPUB Indexes – index-xref-related property]]" ;
                                            rdfs:comment "Reference from one term to one or more related terms or term categories in an index (analogous to \"See also xxx\")." .

:index-term-category                        a rdf:Property ;
                                            jena:prop-sort "140" ;
                                            rdfs:label "index-term-category" ;
                                            rdf:member :indexes ;
                                            role:scope :index-xref-preferred ;
                                            role:scope :index-xref-related ;
                                            htu:usage "[[http://www.w3.org/TR/html5/text-level-semantics.html#the-a-element a]]" ;
                                            epub:usage "[[http://www.idpf.org/epub/idx/epub-indexes.html#bb-term-category EPUB Indexes – index-term-category property]]" ;
                                            rdfs:comment "Word, phrase, string, glyph or image representing a category of terms in the index." .

:index-term-categories                      a rdf:Property ;
                                            jena:prop-sort "150" ;
                                            rdfs:label "index-term-categories" ;
                                            rdf:member :indexes ;
                                            role:scope :index-xref-preferred ;
                                            role:scope :index-xref-related ;
                                            htu:usage "[[http://www.w3.org/TR/html5/text-level-semantics.html#the-a-element a]]" ;
                                            epub:usage "[[http://www.idpf.org/epub/idx/epub-indexes.html#bb-term-categories EPUB Indexes – index-term-categories property]]" ;
                                            rdfs:comment "Wrapper for a list of the term categories belonging to an index." .


########## glossaries #########

:glossaries                                 a rdf:Bag ;
                                            jena:bag-sort "43" ;
                                            rdf:member :references ;
                                            dcterms:title "Glossaries" .

:glossary                                   a rdf:Property ;
                                            rdfs:label "glossary" ;
                                            rdf:member :glossaries ;
                                            htu:usage "[[http://www.w3.org/TR/html5/grouping-content.html#the-dl-element dl]], [[http://www.w3.org/TR/html5/dom.html#sectioning-content-0 sectioning content]]" ;
                                            jena:prop-sort "10";
                                            rdfs:comment "A brief dictionary of new, uncommon or specialized terms used in the content." .

:glossterm                                  a rdf:Property ;
                                            rdfs:label "glossterm" ;
                                            rdf:member :glossaries ;
                                            role:scope :glossary ;
                                            htu:usage "When the element on which the property appears is a [[http://www.w3.org/TR/html5/grouping-content.html#the-dt-element dt]] element within a [[http://www.w3.org/TR/html5/grouping-content.html#the-dl-element dl]] element marked with the [[#glossary]] property, then the glossterm property on the given dt element is implied." ;
                                            jena:prop-sort "20";
                                            rdfs:comment "A glossary term." .
					
:glossdef                                   a rdf:Property ;
                                            rdfs:label "glossdef" ;
                                            role:scope :glossary ;
                                            rdf:member :glossaries ;
                                            htu:usage "When the element on which the property appears a [[http://www.w3.org/TR/html5/grouping-content.html#the-dd-element dd]] element within a [[http://www.w3.org/TR/html5/grouping-content.html#the-dl-element dl]] element marked with the [[#glossary]] property, then the glossdef property on the given dd element is implied. When the element context is a [[http://www.w3.org/TR/html5/sections.html#the-dt-element dd]] element and no explicit glossterm link is provided, then the term that this glossdef participates in defining is located in the nearest preceding [[http://www.w3.org/TR/html5/sections.html#the-dt-element dt]] element sibling. " ;
                                            jena:prop-sort "30";
                                            rdfs:comment "The definition of a [[#glossterm term in a glossary]]." .


########## bibliographies #########

:bibliographies                             a rdf:Bag ;
                                            jena:bag-sort "46" ;
                                            rdf:member :references ;
                                            dcterms:title "Bibliographies" .

:bibliography                               a rdf:Property ;
                                            rdfs:label "bibliography" ;
                                            rdf:member :bibliographies ;
                                            htu:usage "[[http://www.w3.org/TR/html5/dom.html#sectioning-content-0 sectioning content]]" ;
                                            jena:prop-sort "10" ;
                                            rdfs:comment "A list of external references cited in the work, which may be to print or digital sources." .

:biblioentry                                a rdf:Property ;
                                            rdfs:label "biblioentry" ;
                                            rdf:member :bibliographies ;
                                            role:scope :bibliography ;
                                            htu:usage "[[http://www.w3.org/TR/html5/grouping-content.html#grouping-content grouping content]]" ;
                                            jena:prop-sort "20" ;
                                            rdfs:comment "A single reference to an external source in a [[#bibliography]]. A biblioentry typically provides more detailed information than its reference(s) in the content (e.g., full title, author(s), publisher, publication date, etc.)." .


########## preliminary #########

:preliminary                                a rdf:Bag ;
                                            jena:bag-sort "50" ;
                                            dcterms:title "Preliminary sections and components" ;
                                            dcterms:description "Preliminary sections and components, typically occuring in the publication frontmatter." .

:titlepage                                  a rdf:Property ;
                                            rdfs:label "titlepage" ;
                                            rdf:member :preliminary ;
                                            htu:usage "[[http://www.w3.org/TR/html5/sections.html#the-section-element section]], [[http://www.w3.org/TR/html5/grouping-content.html#grouping-content grouping content]]" ;
                                            jena:prop-sort "10" ;
                                            rdfs:comment "The title page of the work." .

:halftitlepage                              a rdf:Property ;
                                            rdfs:label "halftitlepage" ;
                                            rdf:member :preliminary ;
                                            htu:usage "[[http://www.w3.org/TR/html5/sections.html#the-section-element section]], [[http://www.w3.org/TR/html5/grouping-content.html#grouping-content grouping content]]" ;
                                            jena:prop-sort "20" ;
                                            rdfs:comment "The half title page of the work." .

:copyright-page                             a rdf:Property ;
                                            rdfs:label "copyright-page" ;
                                            rdf:member :preliminary ;
                                            htu:usage "[[http://www.w3.org/TR/html5/sections.html#the-section-element section]], [[http://www.w3.org/TR/html5/grouping-content.html#grouping-content grouping content]]" ;
                                            jena:prop-sort "30" ;
                                            rdfs:comment "The copyright page of the work." .

:seriespage                                 a rdf:Property ;
                                            rdfs:label "seriespage " ;
                                            rdf:member :preliminary ;
                                            htu:usage "[[http://www.w3.org/TR/html5/sections.html#the-section-element section]], [[http://www.w3.org/TR/html5/grouping-content.html#grouping-content grouping content]]" ;
                                            jena:prop-sort "35" ;
                                            rdfs:comment "Marketing section used to list related publications." ;
                                            epub:status "draft" .

:acknowledgments                            a rdf:Property ;
                                            rdfs:label "acknowledgments" ;
                                            rdf:member :preliminary ;
                                            htu:usage "[[http://www.w3.org/TR/html5/sections.html#the-section-element section]], [[http://www.w3.org/TR/html5/grouping-content.html#grouping-content grouping content]]" ;
                                            jena:prop-sort "40" ;
                                            rdfs:comment "A section or statement that acknowledges significant contributions by persons, organizations, governments and other entities to the realization of the work." .

:imprint                                    a rdf:Property ;
                                            rdfs:label "imprint" ;
                                            rdf:member :preliminary ;
                                            htu:usage "[[http://www.w3.org/TR/html5/sections.html#the-section-element section]], [[http://www.w3.org/TR/html5/grouping-content.html#grouping-content grouping content]]" ;
                                            jena:prop-sort "50" ;
                                            rdfs:comment "Information relating to the publication or distribution of the work." .

:imprimatur                                 a rdf:Property ;
                                            rdfs:label "imprimatur" ;
                                            rdf:member :preliminary ;
                                            htu:usage "[[http://www.w3.org/TR/html5/sections.html#the-section-element section]], [[http://www.w3.org/TR/html5/grouping-content.html#grouping-content grouping content]]" ;
                                            jena:prop-sort "60" ;
                                            rdfs:comment "A formal statement authorizing the publication of the work." .

:contributors                               a rdf:Property ;
                                            rdfs:label "contributors" ;
                                            rdf:member :preliminary ;
                                            htu:usage "[[http://www.w3.org/TR/html5/sections.html#the-section-element section]], [[http://www.w3.org/TR/html5/grouping-content.html#grouping-content grouping content]]" ;
                                            jena:prop-sort "70" ;
                                            rdfs:comment "A list of contributors to the work." .

:other-credits                              a rdf:Property ;
                                            rdfs:label "other-credits" ;
                                            rdf:member :preliminary ;
                                            htu:usage "[[http://www.w3.org/TR/html5/sections.html#the-section-element section]], [[http://www.w3.org/TR/html5/grouping-content.html#grouping-content grouping content]]" ;
                                            jena:prop-sort "80" ;
                                            rdfs:comment "Acknowledgments of previously published parts of the work, illustration credits, and permission to quote from copyrighted material." .

:errata                                     a rdf:Property ;
                                            rdfs:label "errata" ;
                                            rdf:member :preliminary ;
                                            htu:usage "[[http://www.w3.org/TR/html5/sections.html#the-section-element section]], [[http://www.w3.org/TR/html5/sections.html#the-aside-element aside]], [[http://www.w3.org/TR/html5/grouping-content.html#grouping-content grouping content]]" ;
                                            jena:prop-sort "90" ;
                                            rdfs:comment "A set of corrections discovered after initial publication of the work, sometimes referred to as corrigenda." .

:dedication                                 a rdf:Property ;
                                            rdfs:label "dedication" ;
                                            rdf:member :preliminary ;
                                            htu:usage "[[http://www.w3.org/TR/html5/sections.html#the-section-element section]], [[http://www.w3.org/TR/html5/grouping-content.html#grouping-content grouping content]]" ;
                                            jena:prop-sort "100" ;
                                            rdfs:comment "An inscription at the front of the work, typically addressed in tribute to one or more persons close to the author." .

:revision-history                           a rdf:Property ;
                                            rdfs:label "revision-history" ;
                                            rdf:member :preliminary ;
                                            htu:usage "[[http://www.w3.org/TR/html5/sections.html#the-section-element section]], [[http://www.w3.org/TR/html5/grouping-content.html#grouping-content grouping content]]" ;
                                            jena:prop-sort "110" ;
                                            rdfs:comment "A record of changes made to a work." .



############ complementary ##########

:asides                                     a rdf:Bag ;
                                            jena:bag-sort "60" ;
                                            dcterms:title "Complementary content" .

:case-study                                 a rdf:Property ;
                                            rdfs:label "case-study" ;
                                            rdfs:subPropertyOf xhv:complementary ;
                                            rdf:member :asides ;
                                            htu:usage "[[http://www.w3.org/TR/html5/dom.html#sectioning-content-0 sectioning content]]" ;
                                            jena:prop-sort "5" ;
                                            rdfs:comment "A detailed analysis of a specific topic." ;
                                            epub:status "draft" .

:help                                       a rdf:Property ;
                                            rdfs:label "help" ;
                                            rdfs:subPropertyOf xhv:complementary ;
                                            rdf:member :asides ;
                                            htu:usage "[[http://www.w3.org/TR/html5/sections.html#the-aside-element aside]], [[http://www.w3.org/TR/html5/dom.html#phrasing-content phrasing content]]" ;
                                            jena:prop-sort "10" ;
                                            rdfs:comment "Helpful information that clarifies some aspect of the content or assists in its comprehension." .

:marginalia                                 a rdf:Property ;
                                            rdfs:label "marginalia" ;
                                            rdfs:subPropertyOf xhv:complementary ;
                                            rdf:member :asides ;
                                            htu:usage "[[http://www.w3.org/TR/html5/sections.html#the-aside-element aside]], [[http://www.w3.org/TR/html5/dom.html#phrasing-content phrasing content]]" ;
                                            jena:prop-sort "20" ;
                                            rdfs:comment "Content, both textual and graphical, that is offset in the margin." ;
                                            owl:deprecated "true" ;
                                            dcterms:isReplacedBy "[[http://www.w3.org/TR/html5/sections.html#the-aside-element aside]]".

:notice                                     a rdf:Property ;
                                            rdfs:label "notice" ;
                                            rdf:member :asides ;
                                            htu:usage "[[http://www.w3.org/TR/html5/sections.html#the-section-element section]], [[http://www.w3.org/TR/html5/grouping-content.html#grouping-content grouping content]]" ;
                                            jena:prop-sort "30" ;
                                            rdfs:comment "Notifies the user of consequences that might arise from an action or event. Examples include warnings, cautions and dangers." .

:pullquote                                  a rdf:Property ;
                                            rdfs:label "pullquote" ;
                                            rdfs:subPropertyOf xhv:complementary ;
                                            rdf:member :asides ;
                                            htu:usage "[[http://www.w3.org/TR/html5/sections.html#the-aside-element aside]]" ;
                                            jena:prop-sort "40" ;
                                            rdfs:comment "A distinctively placed or highlighted quotation from the current content designed to draw attention to a topic or highlight a key point." ;
                                            epub:status "draft" .

:sidebar                                    a rdf:Property ;
                                            rdfs:label "sidebar" ;
                                            rdfs:subPropertyOf xhv:complementary ;
                                            rdf:member :asides ;
                                            htu:usage "[[http://www.w3.org/TR/html5/sections.html#the-aside-element aside]]" ;
                                            jena:prop-sort "50" ;
                                            rdfs:comment "Secondary or supplementary content, typically formatted as an inset or box." ;
                                            owl:deprecated "true" ;
                                            dcterms:isReplacedBy "[[http://www.w3.org/TR/html5/sections.html#the-aside-element aside]]".

:warning                                    a rdf:Property ;
                                            rdfs:label "warning" ;
                                            rdf:member :asides ;
                                            htu:usage "[[http://www.w3.org/TR/html5/sections.html#the-section-element section]], [[http://www.w3.org/TR/html5/grouping-content.html#grouping-content grouping content]]" ;
                                            jena:prop-sort "60" ;
                                            rdfs:comment "A warning." ;
                                            owl:deprecated "true" ;
                                            dcterms:isReplacedBy "[[#notice]]".



############### titles ##############
:titles                                     a rdf:Bag ;
                                            jena:bag-sort "70" ;
                                            dcterms:title "Titles and headings" .

:halftitle                                  a rdf:Property ;
                                            rdfs:label "halftitle" ;
                                            rdfs:subPropertyOf :title ;
                                            rdf:member :titles ;
                                            htu:usage "[[http://www.w3.org/TR/html5/dom.html#heading-content heading content]]. This property should only appear once within the document scope." ;
                                            jena:prop-sort "10" ;
                                            rdfs:comment "The title appearing on the first page of a work or immediately before the text." .

:fulltitle                                  a rdf:Property ;
                                            rdfs:label "fulltitle" ;
                                            rdfs:subPropertyOf :title ;
                                            rdf:member :titles ;
                                            owl:sameAs dcterms:title;
                                            htu:usage "[[http://www.w3.org/TR/html5/dom.html#heading-content heading content]]. This property should only appear once within the document scope." ;
                                            jena:prop-sort "20" ;
                                            rdfs:comment "The full title of the work, either simple, in which case it is identical to [[#title]], or compound, in which case it consists of a [[#title]] and a [[#subtitle]]." .

:covertitle                                 a rdf:Property;
                                            rdfs:label "covertitle" ;
                                            rdfs:subPropertyOf :title ;
                                            rdf:member :titles ;
                                            htu:usage "[[http://www.w3.org/TR/html5/dom.html#heading-content heading content]]. This property should only appear once within the document scope." ;
                                            jena:prop-sort "30"; 
                                            rdfs:comment "The title of the work as displayed on the work's cover." .

:title                                      a rdf:Property ;
                                            rdfs:label "title" ;
                                            rdf:member :titles ;
                                            htu:usage "[[http://www.w3.org/TR/html5/dom.html#heading-content heading content]], [[http://www.w3.org/TR/html5/dom.html#phrasing-content phrasing content]] descendants of [[http://www.w3.org/TR/html5/dom.html#heading-content heading content]]." ;
                                            jena:prop-sort "40";
                                            rdfs:comment "The primary name of a document component, such as a list, table or figure." .

:subtitle                                   a rdf:Property;
                                            rdfs:label "subtitle" ;
                                            rdfs:subPropertyOf :title ;
                                            rdf:member :titles ;
                                            htu:usage "[[http://www.w3.org/TR/html5/dom.html#heading-content heading content]], [[http://www.w3.org/TR/html5/dom.html#phrasing-content phrasing content]] descendants of [[http://www.w3.org/TR/html5/dom.html#heading-content heading content]], [[http://www.w3.org/TR/html5/grouping-content.html#the-p-element paragraphs]], [[http://www.w3.org/TR/html5/grouping-content.html#the-div-element divs]]" ;
                                            jena:prop-sort "50";
                                            rdfs:comment "An explanatory or alternate title for the work, or a section or component within it." .

:label                                      a rdf:Property ;
                                            rdfs:label "label" ;
                                            rdfs:subPropertyOf :title ;
                                            rdf:member :titles ;
                                            htu:usage "[[http://www.w3.org/TR/html5/dom.html#heading-content heading content]], [[http://www.w3.org/TR/html5/grouping-content.html#the-li-element li]], [[http://www.w3.org/TR/html5/grouping-content.html#the-figcaption-element figcaption]]" ;
                                            jena:prop-sort "60";
                                            rdfs:comment "The text label that precedes an [[#ordinal]] in a component title (e.g., 'Chapter', 'Part', 'Figure', 'Table')." ;
                                            epub:status "draft" .

:ordinal                                    a rdf:Property;
                                            rdfs:label "ordinal" ;
                                            rdfs:subPropertyOf :title ;
                                            rdf:member :titles ;
                                            htu:usage "[[http://www.w3.org/TR/html5/dom.html#heading-content heading content]], [[http://www.w3.org/TR/html5/grouping-content.html#the-li-element li]], [[http://www.w3.org/TR/html5/grouping-content.html#the-figcaption-element figcaption]]" ;
                                            jena:prop-sort "70";
                                            rdfs:comment "An ordinal specifier for a component in a sequence of components (e.g., '1', 'IV', 'B-1')." ;
                                            epub:status "draft" .

:bridgehead                                 a rdf:Property;
                                            rdfs:label "bridgehead" ;
                                            rdf:member :titles ;
                                            htu:usage "[[http://www.w3.org/TR/html5/rendering.html#flow-content-0 flow content]], typically [[http://www.w3.org/TR/html5/grouping-content.html#the-p-element p]], [[http://www.w3.org/TR/html5/grouping-content.html#the-div-element div]] or [[http://www.w3.org/TR/html5/text-level-semantics.html#the-span-element span]]" ;
                                            jena:prop-sort "80" ;
                                            rdfs:comment "A structurally insignificant heading that does not contribute to the hierarchical structure of the work." .


########## educational ###########


:educational                                a rdf:Bag ;
                                            jena:bag-sort "80" ;
                                            dcterms:title "Educational content" .

########## learning-objectives ###########

:learning-obj                               a rdf:Bag ;
                                            jena:bag-sort 82 ;
                                            rdf:member :educational ;
                                            dcterms:title "Learning objectives" .

:learning-objective                         a rdf:Property ;
                                            rdfs:label "learning-objective" ;
                                            rdf:member :learning-obj ;
                                            htu:usage "[[http://www.w3.org/TR/html5/rendering.html#flow-content-0 flow content]], [[http://www.w3.org/TR/html5/dom.html#phrasing-content phrasing content]]" ;
                                            jena:prop-sort "10" ;
                                            rdfs:comment "An explicit designation or description of a learning objective or a reference to an explicit learning objective." .

:learning-objectives                        a rdf:Property ;
                                            rdfs:label "learning-objectives" ;
                                            rdf:member :learning-obj ;
                                            htu:usage "[[http://www.w3.org/TR/html5/dom.html#sectioning-content-0 sectioning content]], [[http://www.w3.org/TR/html5/grouping-content.html#grouping-content grouping content]]" ;
                                            jena:prop-sort "20" ;
                                            rdfs:comment "A collection of [[#learning-objective learning-objectives]]." ;
                                            epub:status "draft" .

:learning-outcome                           a rdf:Property ;
                                            rdfs:label "learning-outcome" ;
                                            rdf:member :learning-obj ;
                                            htu:usage "[[http://www.w3.org/TR/html5/rendering.html#flow-content-0 flow content]]" ;
                                            jena:prop-sort "30" ;
                                            rdfs:comment "The understanding or ability a student is expected to achieve as a result of a lesson or activity." ;
                                            epub:status "draft" .

:learning-outcomes                          a rdf:Property ;
                                            rdfs:label "learning-outcomes" ;
                                            rdf:member :learning-obj ;
                                            htu:usage "[[http://www.w3.org/TR/html5/dom.html#sectioning-content-0 sectioning content]], [[http://www.w3.org/TR/html5/grouping-content.html#grouping-content grouping content]]" ;
                                            jena:prop-sort "40" ;
                                            rdfs:comment "A collection of [[#learning-outcome learing-outcomes]]." ;
                                            epub:status "draft" .

:learning-resource                          a rdf:Property ;
                                            rdfs:label "learning-resource" ;
                                            rdf:member :learning-obj ;
                                            htu:usage "[[http://www.w3.org/TR/html5/rendering.html#flow-content-0 flow content]]" ;
                                            jena:prop-sort "50" ;
                                            rdfs:comment "A resource provided to enhance learning, or a reference to such a resource." .

:learning-resources                         a rdf:Property ;
                                            rdfs:label "learning-resources" ;
                                            rdf:member :learning-obj ;
                                            htu:usage "[[http://www.w3.org/TR/html5/dom.html#sectioning-content-0 sectioning content]], [[http://www.w3.org/TR/html5/grouping-content.html#grouping-content grouping content]]" ;
                                            jena:prop-sort "60" ;
                                            rdfs:comment "A collection of [[#learning-resource learning-resources]]." ;
                                            epub:status "draft" .

:learning-standard                          a rdf:Property ;
                                            rdfs:label "learning-standard" ;
                                            rdf:member :learning-obj ;
                                            htu:usage "[[http://www.w3.org/TR/html5/dom.html#sectioning-content-0 sectioning content]], [[http://www.w3.org/TR/html5/dom.html#phrasing-content phrasing content]]" ;
                                            jena:prop-sort "70" ;
                                            rdfs:comment "A formal set of expectations or requirements typically issued by a government or a standards body." ;
                                            epub:status "draft" .

:learning-standards                         a rdf:Property ;
                                            rdfs:label "learning-standards" ;
                                            rdf:member :learning-obj ;
                                            htu:usage "[[http://www.w3.org/TR/html5/dom.html#sectioning-content-0 sectioning content]], [[http://www.w3.org/TR/html5/grouping-content.html#grouping-content grouping content]]" ;
                                            jena:prop-sort "80" ;
                                            rdfs:comment "A collection of [[#learning-standard learning-standards]]." ;
                                            epub:status "draft" .


########### testing #############

:testing                                    a rdf:Bag ;
                                            jena:bag-sort 84 ;
                                            rdf:member :educational ;
                                            dcterms:title "Testing" .

:answer                                     a rdf:Property ;
                                            rdfs:label "answer";
                                            rdf:member :testing ;
                                            htu:usage "[[http://www.w3.org/TR/html5/sections.html#the-aside-element aside]], [[http://www.w3.org/TR/html5/grouping-content.html#grouping-content grouping content]]" ;
                                            jena:prop-sort "10" ;
                                            rdfs:comment "The component of a self-assessment problem that provides the answer to the question." ;
                                            epub:status "draft" .

:answers                                    a rdf:Property ;
                                            rdfs:label "answers";
                                            rdf:member :testing ;
                                            htu:usage "[[http://www.w3.org/TR/html5/dom.html#sectioning-content-0 sectioning content]], [[http://www.w3.org/TR/html5/grouping-content.html#grouping-content grouping content]]" ;
                                            jena:prop-sort "20" ;
                                            rdfs:comment "A collection of [[#answer answers]]." ;
                                            epub:status "draft" .

:assessment                                 a rdf:Property ;
                                            rdfs:label "assessment" ;
                                            rdf:member :testing ;
                                            htu:usage "[[http://www.w3.org/TR/html5/dom.html#sectioning-content-0 sectioning content]]" ;
                                            jena:prop-sort "30" ;
                                            rdfs:comment "A test, quiz, or other activity that helps measure a student's understanding of what is being taught." .

:assessments                                a rdf:Property ;
                                            rdfs:label "assessments" ;
                                            rdf:member :testing ;
                                            htu:usage "[[http://www.w3.org/TR/html5/dom.html#sectioning-content-0 sectioning content]]" ;
                                            jena:prop-sort "40" ;
                                            rdfs:comment "A collection of [[#assessment assessments]]." ;
                                            epub:status "draft" .

:feedback                                   a rdf:Property ;
                                            rdfs:label "feedback";
                                            rdf:member :testing ;
                                            htu:usage "[[http://www.w3.org/TR/html5/grouping-content.html#grouping-content grouping content]], [[http://www.w3.org/TR/html5/dom.html#phrasing-content phrasing content]]" ;
                                            jena:prop-sort "50" ;
                                            rdfs:comment "Instruction to the reader based on the result of an assessment." ;
                                            epub:status "draft" .

:fill-in-the-blank-problem                  a rdf:Property ;
                                            rdfs:label "fill-in-the-blank-problem";
                                            rdf:member :testing ;
                                            htu:usage "[[http://www.w3.org/TR/html5/sections.html#the-aside-element aside]], [[http://www.w3.org/TR/html5/grouping-content.html#grouping-content grouping content]]" ;
                                            jena:prop-sort "60" ;
                                            rdfs:comment "A problem that requires the reader to input a text answer to complete a sentence, statement or similar." ;
                                            epub:status "draft" .

:general-problem                            a rdf:Property ;
                                            rdfs:label "general-problem";
                                            rdf:member :testing ;
                                            htu:usage "[[http://www.w3.org/TR/html5/sections.html#the-aside-element aside]], [[http://www.w3.org/TR/html5/grouping-content.html#grouping-content grouping content]]" ;
                                            jena:prop-sort "70" ;
                                            rdfs:comment "A problem with a free-form solution." ;
                                            epub:status "draft" .

:match-problem                              a rdf:Property ;
                                            rdfs:label "match-problem";
                                            rdf:member :testing ;
                                            htu:usage "[[http://www.w3.org/TR/html5/sections.html#the-aside-element aside]], [[http://www.w3.org/TR/html5/grouping-content.html#grouping-content grouping content]]" ;
                                            jena:prop-sort "80" ;
                                            rdfs:comment "A problem that requires the reader to match the contents of one list with the corresponding items in another list." ;
                                            epub:status "draft" .

:multiple-choice-problem                    a rdf:Property ;
                                            rdfs:label "multiple-choice-problem";
                                            rdf:member :testing ;
                                            htu:usage "[[http://www.w3.org/TR/html5/sections.html#the-aside-element aside]], [[http://www.w3.org/TR/html5/grouping-content.html#grouping-content grouping content]]" ;
                                            jena:prop-sort "90" ;
                                            rdfs:comment "A problem with a set of potential answers to choose from ‒ some, all or none of which may be correct." ;
                                            epub:status "draft" .

:practice                                   a rdf:Property ;
                                            rdfs:label "practice" ;
                                            rdf:member :testing ;
                                            rdfs:seeAlso :practices;
                                            htu:usage "[[http://www.w3.org/TR/html5/sections.html#the-aside-element aside]], [[http://www.w3.org/TR/html5/grouping-content.html#grouping-content grouping content]]" ;
                                            jena:prop-sort "100" ;
                                            rdfs:comment "A review exercise or sample." ;
                                            epub:status "draft" .

:practices                                  a rdf:Property ;
                                            rdfs:label "practices" ;
                                            rdf:member :testing ;
                                            htu:usage "[[http://www.w3.org/TR/html5/dom.html#sectioning-content-0 sectioning content]]" ;
                                            jena:prop-sort "110" ;
                                            rdfs:comment "A collection of [[#practice practices]]." ;
                                            epub:status "draft" .

:question                                   a rdf:Property ;
                                            rdfs:label "question" ;
                                            rdf:member :testing ;
                                            htu:usage "[[http://www.w3.org/TR/html5/grouping-content.html#grouping-content grouping content]]" ;
                                            jena:prop-sort "110" ;
                                            rdfs:comment "The component of a self-assessment problem that identifies the question to be solved." ;
                                            epub:status "draft" .

:true-false-problem                         a rdf:Property ;
                                            rdfs:label "true-false-problem";
                                            rdf:member :testing ;
                                            htu:usage "[[http://www.w3.org/TR/html5/sections.html#the-aside-element aside]], [[http://www.w3.org/TR/html5/grouping-content.html#grouping-content grouping content]]" ;
                                            jena:prop-sort "130" ;
                                            rdfs:comment "A problem with either a true or false answer." ;
                                            epub:status "draft" .



############# comics ##############

:comics                                     a rdf:Bag ;
                                            jena:bag-sort "87" ;
                                            dcterms:title "Comics" .

:panel                                      a rdf:Property ;
                                            rdfs:label "panel" ;
                                            rdf:member :comics ;
                                            jena:prop-sort "5" ;
                                            htu:usage "[[http://www.w3.org/TR/html5/grouping-content.html#the-li-element li]]" ;
                                            epub:usage "[[http://www.idpf.org/epub/renditions/region-nav EPUB Region-Based Navigation]]" ;
                                            rdfs:comment "An individual frame, or drawing." .

:panel-group                                a rdf:Property ;
                                            rdfs:label "panel-group" ;
                                            rdf:member :comics ;
                                            jena:prop-sort "10" ;
                                            htu:usage "[[http://www.w3.org/TR/html5/grouping-content.html#the-li-element li]]" ;
                                            epub:usage "[[http://www.idpf.org/epub/renditions/region-nav EPUB Region-Based Navigation]]" ;
                                            rdfs:comment "A group of [[#panel panels]] (e.g., a strip)." .

:balloon                                    a rdf:Property ;
                                            rdfs:label "balloon" ;
                                            rdf:member :comics ;
                                            jena:prop-sort "15" ;
                                            htu:usage "[[http://www.w3.org/TR/html5/grouping-content.html#the-li-element li]]" ;
                                            epub:usage "[[http://www.idpf.org/epub/renditions/region-nav EPUB Region-Based Navigation]]" ;
                                            rdfs:comment "An area in a comic [[#panel panel]] that contains the words, spoken or thought, of a character." .

:text-area                                  a rdf:Property ;
                                            rdfs:label "text-area" ;
                                            rdf:member :comics ;
                                            jena:prop-sort "20" ;
                                            htu:usage "[[http://www.w3.org/TR/html5/grouping-content.html#the-li-element li]]" ;
                                            epub:usage "[[http://www.idpf.org/epub/renditions/region-nav EPUB Region-Based Navigation]]" ;
                                            rdfs:comment "An area of text in a comic [[#panel panel]]. Used to represent titles, narrative text, character dialogue (inside a [[#balloon balloon]] or not) and similar." .

:sound-area                                 a rdf:Property ;
                                            rdfs:label "sound-area" ;
                                            rdf:member :comics ;
                                            jena:prop-sort "25" ;
                                            htu:usage "[[http://www.w3.org/TR/html5/grouping-content.html#the-li-element li]]" ;
                                            epub:usage "[[http://www.idpf.org/epub/renditions/region-nav EPUB Region-Based Navigation]]" ;
                                            rdfs:comment "An area of text in a comic [[#panel panel]] that represents a sound." .

############# notes ##############

:notes                                      a rdf:Bag ;
                                            jena:bag-sort "90" ;
                                            dcterms:title "Notes and annotations" .

:annotation                                 a rdf:Property ;
                                            rdfs:label "annotation" ;
                                            rdfs:subPropertyOf xhv:complementary ;
                                            rdf:member :notes ;
                                            jena:prop-sort "5" ;
                                            htu:usage "[[http://www.w3.org/TR/html5/sections.html#the-aside-element aside]], [[http://www.w3.org/TR/html5/dom.html#phrasing-content phrasing content]]" ;
                                            rdfs:comment "Explanatory information about passages in the work." ;
                                            owl:deprecated "true" ;
                                            dcterms:isReplacedBy "[[http://www.idpf.org/epub/oa Open Annotation in EPUB]]".

:note                                       a rdf:Property ;
                                            rdfs:label "note" ;
                                            rdf:member :notes ;
                                            htu:usage "On the [[http://www.w3.org/TR/html5/sections.html#the-aside-element aside]] element when identifying a single note, or on descendants of sectioning content when identifying individual notes in a group (refer to [[#footnotes footnotes]] and [[#rearnotes rearnotes]])." ;
                                            jena:prop-sort "10" ;
                                            rdfs:comment "A note. This property does not carry spatial positioning semantics, as do the [[#footnote]] and [[#rearnote]] properties. It can be used to identify footnotes, rear notes, marginal notes, inline notes, and similar when legacy naming conventions are not desired." ;
                                            owl:deprecated "true" ;
                                            dcterms:isReplacedBy "[[#footnote]], [[#rearnote]]".

:footnote                                   a rdf:Property ;
                                            rdfs:label "footnote" ;
                                            rdf:member :notes ;
                                            rdfs:seeAlso :footnotes;
                                            htu:usage "On the [[http://www.w3.org/TR/html5/sections.html#the-aside-element aside]] element when identifying a single footnote, or on descendants of sectioning content when identifying individual footnotes in a group (refer to [[#footnotes footnotes]] and [[#rearnotes rearnotes]]). " ;
                                            jena:prop-sort "20" ;
                                            rdfs:comment "Ancillary information, such as a citation or commentary, that provides additional context to a referenced passage of text." .

:rearnote                                   a rdf:Property ;
                                            rdfs:label "rearnote" ;
                                            rdf:member :notes ;
                                            rdfs:seeAlso :rearnotes;
                                            htu:usage "On the [[http://www.w3.org/TR/html5/sections.html#the-aside-element aside]] element when identifying a single rearnote, or on descendants of sectioning content when identifying individual rearnotes in a group (refer to [[#footnotes footnotes]] and [[#rearnotes rearnotes]])." ;
                                            jena:prop-sort "30" ;
                                            rdfs:comment "A note appearing in the rear (backmatter) of the work, or at the end of a section." .


:footnotes                                  a rdf:Property ;
                                            rdfs:label "footnotes" ;
                                            rdfs:seeAlso :footnote;
                                            rdf:member :notes ;
                                            htu:usage "[[http://www.w3.org/TR/html5/dom.html#sectioning-content-0 sectioning content]]" ;
                                            jena:prop-sort "40" ;
                                            rdfs:comment "A collection of [[#footnote footnotes]]." .

:rearnotes                                  a rdf:Property ;
                                            rdfs:label "rearnotes" ;
                                            rdf:member :notes ;
                                            rdfs:seeAlso :rearnote ;
                                            htu:usage "[[http://www.w3.org/TR/html5/dom.html#sectioning-content-0 sectioning content]]" ;
                                            jena:prop-sort "50" ;
                                            rdfs:comment "A collection of notes appearing at the rear (backmatter) of the work, or at the end of a section." .


############# references ###############


:links                                      a rdf:Bag ;
                                            jena:bag-sort "95" ;
                                            dcterms:title "References" .

:annoref                                    a rdf:Property ;
                                            rdfs:label "annoref" ;
                                            rdfs:subPropertyOf xhv:link ;
                                            rdf:member :links ;
                                            htu:usage "[[http://www.w3.org/TR/html5/text-level-semantics.html#the-a-element a]]" ;
                                            rdfs:comment "A reference to an annotation." ;
                                            jena:prop-sort "10" ;
                                            rdfs:seeAlso :annotation ;
                                            owl:deprecated "true" ;
                                            dcterms:isReplacedBy "[[http://www.idpf.org/epub/oa Open Annotation in EPUB]]".

:biblioref                                  a rdf:Property ;
                                            rdfs:label "biblioref" ;
                                            rdfs:subPropertyOf xhv:link ;
                                            rdf:member :links ;
                                            htu:usage "[[http://www.w3.org/TR/html5/text-level-semantics.html#the-a-element a]]" ;
                                            rdfs:comment "A reference to a [[#biblioentry bibliography entry]]." ;
                                            jena:prop-sort "20" ;
                                            epub:status "draft" .

:glossref                                   a rdf:Property ;
                                            rdfs:label "glossref" ;
                                            rdfs:subPropertyOf xhv:link ;
                                            rdf:member :links ;
                                            htu:usage "[[http://www.w3.org/TR/html5/text-level-semantics.html#the-a-element a]]" ;
                                            rdfs:comment "A reference to a [[#glossdef glossary definition]]." ;
                                            jena:prop-sort "30" ;
                                            epub:status "draft" .

:noteref                                    a rdf:Property ;
                                            rdfs:label "noteref" ;
                                            rdfs:subPropertyOf xhv:link ;
                                            rdf:member :links ;
                                            htu:usage "[[http://www.w3.org/TR/html5/text-level-semantics.html#the-a-element a]]" ;
                                            rdfs:comment "A reference to a note, typically appearing as a superscripted number or symbol in the main body of text." ;
                                            jena:prop-sort "40" ;
                                            rdfs:seeAlso :note .

:referrer                                   a rdf:Property ;
                                            rdfs:label "referrer" ;
                                            rdfs:subPropertyOf xhv:link ;
                                            rdf:member :links ;
                                            htu:usage "[[http://www.w3.org/TR/html5/text-level-semantics.html#the-a-element a]]" ;
                                            rdfs:comment "A link that allows the user to jump to a related location in the content (e.g., from a footnote to its reference, from an index entry to where the topic is discussed, or from a glossary definition to where the term is used)." ;
                                            jena:prop-sort "50" ;
                                            epub:status "draft" .




############# document text #############


:document-text                              a rdf:Bag ;
                                            jena:bag-sort "100" ;
                                            dcterms:title "Document text" ;
                                            dcterms:description "Terms for describing components at the phrasing level." .

:credit                                     a rdf:Property ;
                                            rdfs:label "credit" ;
                                            rdf:member :document-text ;
                                            htu:usage "[[http://www.w3.org/TR/html5/dom.html#phrasing-content phrasing content]]" ;
                                            jena:prop-sort "05" ;
                                            rdfs:comment "An acknowledgment of the source of integrated content from third-party sources, such as photos. Typically identifies the creator, copyright and any restrictions on reuse." ;
                                            epub:status "draft" .

:keyword                                    a rdf:Property ;
                                            rdfs:label "keyword" ;
                                            rdf:member :document-text ;
                                            htu:usage "[[http://www.w3.org/TR/html5/dom.html#phrasing-content phrasing content]]" ;
                                            jena:prop-sort "10" ;
                                            rdfs:comment "A key word or phrase." .


:topic-sentence                             a rdf:Property ;
                                            rdfs:label "topic-sentence" ;
                                            rdf:member :document-text ;
                                            htu:usage "[[http://www.w3.org/TR/html5/dom.html#phrasing-content phrasing content]]" ;
                                            jena:prop-sort "20" ;
                                            rdfs:comment "A phrase or sentence serving as an introductory summary of the containing paragraph." .

:concluding-sentence                        a rdf:Property ;
                                            rdfs:label "concluding-sentence" ;
                                            rdf:member :document-text ;
                                            htu:usage "[[http://www.w3.org/TR/html5/dom.html#phrasing-content phrasing content]]" ;
                                            jena:prop-sort "30" ;
                                            rdfs:comment "A phrase or sentence serving as a concluding summary of the containing paragraph." .



############## pagination ##############


:pagination                                 a rdf:Bag ;
                                            jena:bag-sort "140" ;
                                            dcterms:title "Pagination" .

:pagebreak                                  a rdf:Property ;
                                            rdfs:label "pagebreak" ;
                                            rdf:member :pagination ;
                                            htu:usage "[[http://www.w3.org/TR/html5/dom.html#phrasing-content phrasing]] and [[http://www.w3.org/TR/html5/dom.html#flow-content flow]] content, where the value of the carrying elements title attribute takes precedence over element content for the purposes of representing the pagebreak value" ;
                                            jena:prop-sort "10" ;
                                            rdfs:comment "A separator denoting the position before which a break occurs between two contiguous pages in a statically paginated version of the content." .

:page-list                                  a rdf:Property ;
                                            rdfs:label "page-list" ;
                                            rdf:member :pagination ; 
                                            htu:usage "[[http://www.w3.org/TR/html5/dom.html#sectioning-content-0 sectioning content]]" ;
                                            jena:prop-sort "20" ;
                                            rdfs:comment "A navigational aid that provides a list of links to the [[#pagebreak pagebreaks]] in the content." .



############## tables ##############


:tables                                     a rdf:Bag ;
                                            jena:bag-sort "150" ;
                                            dcterms:title "Tables" .

:table                                      a rdf:Property ;
                                            rdfs:label "table" ;
                                            rdf:member :tables ;
                                            jena:prop-sort "10";
                                            htu:usage "Deprecated"; 
                                            mou:usage "Identifies a [[http://www.idpf.org/epub/latest/mediaoverlays#sec-smil-seq-elem seq]] or [[http://www.idpf.org/epub/latest/mediaoverlays#sec-smil-par-elem par]] as an escapable or skippable table structure." ;
                                            rdfs:comment "A structure containing data or content laid out in tabular form." .

:table-row                                  a rdf:Property ;
                                            rdfs:label "table-row" ;
                                            rdf:member :tables ;
                                            jena:prop-sort "20";
                                            htu:usage "Deprecated" ;
                                            mou:usage "Identifies a [[http://www.idpf.org/epub/latest/mediaoverlays#sec-smil-seq-elem seq]] or [[http://www.idpf.org/epub/latest/mediaoverlays#sec-smil-par-elem par]] as an escapable or skippable table row." ;
                                            rdfs:comment "A row of data or content in a tabular structure." .

:table-cell                                 a rdf:Property ;
                                            rdfs:label "table-cell" ;
                                            rdf:member :tables ;
                                            jena:prop-sort "30";
                                            htu:usage "Deprecated" ; 
                                            mou:usage "Identifies a [[http://www.idpf.org/epub/latest/mediaoverlays#sec-smil-seq-elem seq]] or [[http://www.idpf.org/epub/latest/mediaoverlays#sec-smil-par-elem par]] as an escapable or skippable table cell." ;
                                            rdfs:comment "A single cell of tabular data or content." .




############## lists ##############


:lists                                      a rdf:Bag ;
                                            jena:bag-sort "160" ;
                                            dcterms:title "Lists" .

:list                                       a rdf:Property ;
                                            rdfs:label "list" ;
                                            rdf:member :lists ;
                                            jena:prop-sort "10";
                                            htu:usage "Deprecated" ;
                                            mou:usage "Identifies a [[http://www.idpf.org/epub/latest/mediaoverlays#sec-smil-seq-elem seq]] or [[http://www.idpf.org/epub/latest/mediaoverlays#sec-smil-par-elem par]] as an escapable or skippable list structure." ;
                                            rdfs:comment "A structure that contains an enumeration of related content items." .

:list-item                                  a rdf:Property ;
                                            rdfs:label "list-item" ;
                                            rdf:member :lists ;
                                            jena:prop-sort "20";
                                            htu:usage "Deprecated" ;
                                            mou:usage "Identifies a [[http://www.idpf.org/epub/latest/mediaoverlays#sec-smil-seq-elem seq]] or [[http://www.idpf.org/epub/latest/mediaoverlays#sec-smil-par-elem par]] as an escapable or skippable list item." ;
                                            rdfs:comment "A single item in an enumeration." .


############## figures ##############


:figures                                    a rdf:Bag ;
                                            jena:bag-sort "170" ;
                                            dcterms:title "Figures" .

:figure                                     a rdf:Property ;
                                            rdfs:label "figure" ;
                                            rdf:member :figures ;
                                            jena:prop-sort "10";
                                            htu:usage "Deprecated" ;
                                            mou:usage "Identifies a [[http://www.idpf.org/epub/latest/mediaoverlays#sec-smil-seq-elem seq]] or [[http://www.idpf.org/epub/latest/mediaoverlays#sec-smil-par-elem par]] as an escapable or skippable figure." ;
                                            rdfs:comment "An illustration, diagram, photo, code listing or similar, referenced from the text of a work, and typically annotated with a title, caption and/or credits." .

